\begin{enumerate}[label=\thechapter.\arabic*,ref=\thechapter.\theenumi]
\numberwithin{equation}{enumi}
\numberwithin{figure}{enumi}
\numberwithin{table}{enumi}
\item 
The $Z$-transform of $X$ is defined as
\begin{align}
M_X(z) = E\sbrak{z^{-X}} = \sum_{k=-\infty}^{\infty}p_X(k)z^{-k}
\end{align}
\item The $n$th moment of $X$ can be expressed as
\begin{align}
\label{eq:mgf-mean}
E\sbrak{X^n}&= \frac{d^nM_{X}(z^{-1})}{dz^n}\vert_{z=1}
\end{align}
\item For a Bernoulli random variable $X$ with success probability $p$,
\begin{align}
M_X(z)= q+pz^{-1}
\end{align}
\item Let 
$X_i$ be i.i.d.  For 
\begin{align}
X &= X_1+X_2+...+X_n,
\\
M_X(z)&=\prod_{=1}^{n}M_{X_i}(z)
\end{align}
\item For a Binomial random variable $X$ with parameters $n,p$,
\begin{align}
\label{eq:mgf-binom}
M_X(z)= \brak{q+pz^{-1}}^n
\end{align}
\item The mean for the Binomial r.v. is
\begin{align}
\label{eq:mean-binom}
E\sbrak{X}= np
\end{align}
\solution
From 
\eqref{eq:mgf-mean}
and 
\eqref{eq:mgf-binom},
\begin{align}
E\sbrak{X} 
&= \frac{d(q + pz)^n}{dz}\vert_{z=1}
\\
&=np(q + pz)^{n-1}|_{z=1}
\\
&= np(q + p)^{n-1}
\end{align}
yielding
\eqref{eq:mean-binom}
\begin{align}
\because p+q=1
\end{align}
\end{enumerate}
